src/Capabilities.v
@@ -32,10 +32,12 @@ End Pact.
 Record Sig (n : string) : Set := {
   paramTy : Ty;               (* this could be a product (i.e. pair) *)
   valueTy : Ty;               (* is TUnit for unmanaged caps *)
+  valueMonoid : Monoid (Value valueTy)
 }.
 
 Arguments paramTy {n} _.
 Arguments valueTy {n} _.
+Arguments valueMonoid {n} _.
 
 Inductive Cap `(S : Sig n) : Set :=
   | Token : Value (paramTy S) → Cap S.
@@ -104,14 +106,27 @@ Inductive CEval (D : Defs) :
 
   (* with-capability *)
   | Eval_WITH cs ms ms' (C : ACap) (val : Value (valueTy (sig C))) expr :
+    C ∉ cs →
     ∀ def, is_defined D C def →
-    ∀ avail, valueTy (sig C) = TUnit ∨ existT _ C avail ∈ ms →
+    ∀ avail, (valueTy (sig C) = TUnit ∨ existT _ C avail ∈ ms) →
     ∀ is_monoid : Monoid (Value (valueTy (sig C))),
+      is_monoid = valueMonoid (sig C) →
     ∀ remainder, avail = val ⊗ remainder →
     ∀ arg, cap C = Token arg →
     CEval D
       ({ C } ∪ predicate def arg ∪ cs)
       (set_available ms C remainder)
+      expr
+      ({ C } ∪ predicate def arg ∪ cs) ms' →
+    CEval D
+      cs ms
+      (WITH C val expr)
+      cs ms'
+
+  | Eval_WITH_noop cs ms ms' (C : ACap) (val : Value (valueTy (sig C))) expr :
+    C ∈ cs →
+    CEval D
+      cs ms
       expr
       cs ms' →
     CEval D
@@ -126,16 +141,101 @@ Inductive CEval (D : Defs) :
       (REQUIRE C)
       ({ C } ∪ cs) ms
 
-  | Eval_SEQ cs cs' cs'' ms ms' ms'' expr1 expr2 :
+  (* Sequencing of two capability functions. An important thing to note here
+     is that the set of available capabilities cannot be changed by a
+     sequence, but only through the scoping provided by WITH. *)
+  | Eval_SEQ cs ms ms' ms'' expr1 expr2 :
     CEval D
       cs ms
       expr1
-      cs' ms' →
+      cs ms' →
     CEval D
-      cs' ms'
+      cs ms'
       expr2
-      cs'' ms'' →
+      cs ms'' →
     CEval D
       cs ms
       (SEQ expr1 expr2)
-      cs'' ms''.
+      cs ms''.
+
+Require Import Coq.Logic.EqdepFacts.
+Require Import Coq.Logic.FunctionalExtensionality.
+Require Import Coq.Program.Equality.
+
+Import EqNotations.
+
+Lemma unit_dep t (H : t = TUnit) (v : Value t) : v = rew <- H in VUnit.
+Proof.
+  dependent destruction v; inversion H.
+  simpl_eq.
+  reflexivity.
+Qed.
+
+Theorem With_With_Noop D cs (ms ms' : Available) expr
+        (C : ACap) (val : Value (valueTy (sig C)))
+        (single_definition : ∀ def def',
+            is_defined D C def → is_defined D C def' → def = def')
+        (single_avail : ∀ avail avail',
+            existT _ C avail ∈ ms → existT _ C avail' ∈ ms → avail = avail')
+        (monoid_right_inj : ∀ `{Monoid A} (x y y' : A),
+            x ⊗ y = x ⊗ y' → y = y') :
+  (* given that C is an instance of a defined capability *)
+  ∀ def, is_defined D C def →
+  (* and known that C has an argument *)
+  ∀ arg, cap C = Token arg →
+  (* and that C isn't already in scope *)
+  C ∉ cs →
+  (* and given that the capability has been installed *)
+  ∀ avail, valueTy (sig C) = TUnit ∨ existT _ C avail ∈ ms →
+  (* and knowing that the value type is a monoid *)
+  ∀ is_monoid : Monoid (Value (valueTy (sig C))),
+    is_monoid = valueMonoid (sig C) →
+  (* and knowing that the remainder is a subset of the available amount *)
+  ∀ remainder, avail = val ⊗ remainder →
+  (* and provided that [expr] evaluates with the given environment *)
+  CEval D ({ C } ∪ predicate def arg ∪ cs)
+          (set_available ms C remainder) expr
+          ({ C } ∪ predicate def arg ∪ cs) ms' →
+  (* then we state the theorem that WITH is idempotent *)
+  CEval D cs ms (WITH C val (WITH C val expr)) cs ms'
+    ↔ CEval D cs ms (WITH C val expr) cs ms'.
+Proof.
+  split; intros.
+  - inversion H6; subst; clear H6.
+    + apply Eqdep.EqdepTheory.inj_pair2 in H9; subst.
+      eapply Eval_WITH; eauto.
+      rewrite H0 in H20; inversion H20; subst; clear H0 H20.
+      specialize (single_definition def def0 H H12); subst.
+      destruct H2, H13.
+      * pose proof (unit_dep _ H0 remainder).
+        rewrite H3 in H5.
+        pose proof (unit_dep _ H0 remainder0).
+        rewrite H4.
+        now apply H5.
+      * pose proof (unit_dep _ H0 remainder).
+        rewrite H3 in H5.
+        pose proof (unit_dep _ H0 remainder0).
+        rewrite H4.
+        now apply H5.
+      * pose proof (unit_dep _ H2 remainder).
+        rewrite H3 in H5.
+        pose proof (unit_dep _ H2 remainder0).
+        rewrite H4.
+        now apply H5.
+      * specialize (single_avail _ _ H0 H2).
+        specialize (monoid_right_inj _ _ _ _ _ single_avail); subst.
+        now apply H5.
+    + now apply Eqdep.EqdepTheory.inj_pair2 in H12; subst.
+  - inversion H6; subst; clear H6.
+    + apply Eqdep.EqdepTheory.inj_pair2 in H9; subst.
+      eapply Eval_WITH; eauto.
+      rewrite H0 in H20; inversion H20; subst; clear H0 H20.
+      specialize (single_definition def def0 H H12); subst.
+      eapply Eval_WITH_noop; eauto.
+      now apply Constructive_sets.Add_intro2.
+    + apply Eqdep.EqdepTheory.inj_pair2 in H12; subst.
+      eapply Eval_WITH_noop; eauto.
+      now eapply Eval_WITH; eauto.
+Qed.
+
+Print Assumptions With_With_Noop.
